# Axiomatic Semantics

## Intuition

### Logical Layout

> Programmer: "Do what I WANT you to do, not what I TOLD you to do".jpg

We consider the problem of how to prove that a program does what we require of it.

We base a proof system on assertions of the form

$$ \{ A \}c\{ B \} $$

where $A$ and $B$ are assertions and $c$ is a command. 

The interpretation of this notation is: For all states $\sigma$ that satisfy $A$, if the execution of $c$ from state $\sigma$ terminates in state $\sigma'$ ($\langle c, \sigma \rangle \to \sigma'$) then $\sigma'$ satisfies $B$.

## Axiomatic Semantics

### Partial Correctness Assertion

Let $A,B$ be two logical formulas, $\sigma$ be a state satisfying $A$ ($\sigma \vDash A$), and $c$ be a command, a **partial correctness assertion** is of the form $\{A\}c\{B\}$, meaning

$$ \forall \sigma, \sigma' \in \Sigma.((\sigma \vDash A \land \langle c, \sigma \rangle \to \sigma') \Rightarrow \sigma' \vDash B) $$

I.e., any successful (i.e., terminating) execution of $c$ from a state satisfying $A$ ends up in a state satisfying $B$.

- Assume $c$ starts execution with initial state $\sigma$ with $\sigma \vDash A$, if it terminates in $\sigma'$, then $\sigma' \vDash B$.
- It provides logical properties for input-output relationships.
- Partial correctness assertion does not consider cases if $c$ does not stop.
  - If $c$ does not stop, then any $\{A\}c\{B\}$ holds.
  - The pca $\{true\}c\{false\}$ is also valid.
- The assertion $A$ is called the **precondition** and $B$ is called the **postcondition**.

### Total Correctness Assertion

> total correctness assertion = termination + partial correctness assertion

Let $A, B$ be two logical formulas and $c$ be a command, then the **total correctness assertion** is of the form

$$ [A]c[B] $$

which means that

1. The program will terminate.
   - $\forall \sigma \in \Sigma.[\sigma \vDash A \Rightarrow \exists \sigma' \in \Sigma.(\langle c, \sigma \rangle \to \sigma')]$.
2. The execution of $c$ from any state satisfying $A$ will terminate in a state which satisfies $B$.
   - $\forall \sigma,\sigma' \in \Sigma.((\sigma \vDash A \land \langle c, \sigma \rangle \to \sigma') \Rightarrow \sigma' \vDash B)$.



### Bottom Element

We introduce the bottom element $\bot$ to denote **non-termination**.

- $\mathcal{C}\llbracket c \rrbracket (\sigma) \coloneqq \bot$ if $c$ does not terminate on initial state $\sigma$.
- $\mathcal{C}\llbracket c \rrbracket(\bot) \coloneqq \bot$.
- $\bot \vDash A$ for all logical formulas $A$.

With the bottom element, partial correctness assertion is equivalent to

$$ \forall \sigma \in \Sigma.(\sigma \vDash A \Rightarrow \mathcal{C}\llbracket c \rrbracket(\sigma) \vDash B) $$

## An Assertion Language `Assn`

> TL;DR. First-order logic.

We want to reason about boolean expressions and including the quantifiers $\forall i..., \exists i ...$. Therefore we need to extend $\mathbf{Bexp}$ and $\mathbf{Aexp}$ to include integer variables $i$, over which we can quantify.

### Extended Arithmetic Expressions: $\mathbf{Aexpv}$

$$ a \coloncolonequals n \mid X \mid i \mid a_0 + a_1 \mid a_0 - a_1 \mid a_0 \times a_1 $$

where

- $n$ denotes an integer in $\mathbb{Z}$,
- $X$ denotes a location (program variables, $\mathbf{Loc}$),
- $i$ denotes an integer variable (logical variables, $\mathbf{IntVar}$).

### Extended Boolean Assertions: $\mathbf{Assn}$

$$ A \coloncolonequals true \mid false \mid a_0 = a_1 \mid a_0 \le a_1 \mid A_0 \land A_1 \mid A_0 \lor A_1 \mid \neg A \mid A_0 \Rightarrow A_1 \mid \forall i.A \mid \exists i.A $$

where

- $a_0, a_1$ denotes extended arithmetic expressions from $\mathbf{Aexpv}$,
- $i$ denotes an integer variable from $\mathbf{IntVar}$,
- $\land, \lor, \neg$ denotes connectives from propositional logic,
- $\forall, \exists$ denotes quantifiers from first-order logic.

### Free and Bound Variables

- An integer variable $i$ in an assertion is **bound** if it occurs within the scope of an enclosing quantifier $\forall i$ or $\exists i$.
- It is **free** if it is not bound.

Free variables are denoted by $FV(\cdot)$, and $FV$ is defined via well-founded recursion.

- $FV(n) = FV(X) \coloneqq \emptyset$,
- $FV(i) \coloneqq \{i\}$,
- $FV(a_0 + a_1) \coloneqq FV(a_0) \cup FV(a_1)$,
- $FV(a_0 - a_1) \coloneqq FV(a_0) \cup FV(a_1)$,
- $FV(a_0 \times a_1) \coloneqq FV(a_0) \cup FV(a_1)$.
- $FV(true) = FV(false) \coloneqq \emptyset$,
- $FV(a_0 = a_1) = FV(a_0 \le a_1) \coloneq FV(a_0) \cup FV(a_1)$,
- $FV(a_0 \bowtie a_1) \coloneqq FV(a_0) \cup FV(a_1)$, $\bowtie \in \{ \land, \lor, \Rightarrow \}$,
- $FV(\neg A) \coloneqq FV(A)$,
- $FV(\forall i.A) = FV(\exists i.A) \coloneqq FV(A) \backslash \{i\}$.

With this notation of $FV$, let $A$ be an assertion from $\mathbf{Assn}$ and $i$ be an integer variable in $A$,

- $i$ is free if $i \in FV(A)$,
- $i$ is bounded if $i \notin FV(A)$.
- $A$ is closed if $FV(A) = \emptyset$.

### Substitutions

Informally, let $a \in \mathbf{Aexp}$ be an arithmetic expression *without integer variables*, $i$ be an integer variable, $A$ be an assertion s.t. $i \in FV(A)$, then $A[a/i]$ is the assertion obtained by substituting all free occurrences of $i$ in $A$ by $a$.

#### Well-Founded Definition of Substitution

- $n[a/i] \coloneqq n$,
- $X[a/i] \coloneqq X$,
- $j[a/i] \coloneqq j$ if $j \neq i$,
- $j[a/i] \coloneqq a$ if $j = i$,
- $(a_0 \bowtie a_1)[a/i] \coloneqq a_0[a/i] \bowtie a_1[a/i]$ for $\bowtie \in \{ +, - , \times \}$,
- $true[a/i] \coloneqq true$,
- $false[a/i] \coloneqq false$,
- $a_0[a/i] = a_1[a/i] \coloneqq a_0[a/i] = a_1[a/i]$,
- $a_0[a/i] \le a_1[a/i] \coloneqq a_0[a/i] \le a_1[a/i]$,
- $(A_0 \bowtie A_1)[a/i] \coloneqq A_0[a/i] \bowtie A_1[a/i]$ for $\bowtie \in \{ \land, \lor, \Rightarrow \}$,
- $(\neg A)[a/i] \coloneqq \neg (A[a/i])$.
- $(\forall j.A)[a/i] \coloneqq \forall j.(A[a/i])$ if $j \neq i$.
- $(\forall j.A)[a/i] \coloneqq \forall j.A$ if $j = i$.
- $(\exists j.A)[a/i] \coloneqq \exists j.(A[a/i])$ if $j \neq i$.
- $(\exists j.A)[a/i] \coloneqq \exists j.A$ if $j = i$.

We use similar notations for substituting a location $X$.

### Semantics of Assertions

#### Interpretation

An **interpretation** is a function $I: \mathbf{IntVar} \mapsto \mathbb{Z}$ which assigns an integer to each integer variable.

An interpretation *instantiates* every *free* integer variable. From the perspective of substitution,

$$(I[n/i])(j) = \begin{cases}
  n &\quad j = i\\
  I(j) &\quad o.w.
\end{cases}$$

#### The Meaning of Extended Arithmetic Expressions

We define a semantic function $\mathcal{A}v$ which gives the value associated with an arithmetic expression with integer variables in a particular *state* in a particular *interpretation*, written as $\mathcal{A}v\llbracket a \rrbracket(I, \sigma)$

- $\mathcal{A}v\llbracket n \rrbracket(I, \sigma) \coloneqq n$;
- $\mathcal{A}v\llbracket X \rrbracket(I, \sigma) \coloneqq \sigma(X)$;
- $\mathcal{A}v\llbracket i \rrbracket(I, \sigma) \coloneqq I(i)$;
- $\mathcal{A}v\llbracket a_0 \circ a_1 \rrbracket(I, \sigma) \coloneqq \mathcal{A}v\llbracket a_0 \rrbracket(I, \sigma) \circ \mathcal{A}v\llbracket  a_1 \rrbracket(I, \sigma)$ for $\circ \in \{ +, -, \times \}$;

For all arithmetic expressions (without integer variables) $a \in \mathbf{Aexp}$, it holds that

$$ \forall \sigma, I.(\mathcal{A}\llbracket a \rrbracket(\sigma) = \mathcal{A}v\llbracket a \rrbracket(\sigma, I)). $$

#### The Meaning of Extended Boolean Assertions

We extend the notation of $\vDash$ with a certain interpretation $I$.

Let $\sigma$ be a state, $I$ be an interpretation, $A$ be an assertion from $\mathbf{Assn}$, we define $\sigma \vDash^I A$ as "$\sigma$ satisfies $A$ in $I$".

By structural induction on assertions, we define

- $\sigma \vDash^I true$;
- $\sigma \vDash^I (a_0 = a_1)$ if $\mathcal{A}v\llbracket a_0 \rrbracket(I, \sigma) = \mathcal{A}v\llbracket a_1 \rrbracket(I, \sigma)$;
- $\sigma \vDash^I (a_0 \le a_1)$ if $\mathcal{A}v\llbracket a_0 \rrbracket(I, \sigma) \le \mathcal{A}v\llbracket a_1 \rrbracket(I, \sigma)$;
- $\sigma \vDash^I A \land B$ if $\sigma \vDash^I A$ and $\sigma \vDash^I B$;
- $\sigma \vDash^I A \lor B$ if $\sigma \vDash^I A$ or $\sigma \vDash^I B$;
- $\sigma \vDash^I \neg A$ if not $\sigma \vDash^I A$;
- $\sigma \vDash^I A \Rightarrow B$ if (not $\sigma \vDash^I A$) or $\sigma \vDash^I B$;
- $\sigma \vDash^I \forall i.A$ if $\sigma \vDash^{I[n/i]} A$ for *all* $n \in \mathbb{Z}$;
- $\sigma \vDash^I \exists i.A$ if $\sigma \vDash^{I[n/i]} A$ for *some* $n \in \mathbb{Z}$;
- $\bot \vDash^I A$.

##### Some Results

For all (unextended) boolean expressions $b \in \mathbf{Bexp}$, states $\sigma \in \Sigma$ and intepretations $I$,

- $\mathcal{B}\llbracket b \rrbracket(\sigma) = true$ iff $\sigma \vDash^I b$,
- $\mathcal{B}\llbracket b \rrbracket(\sigma) = false$ iff $\sigma \nvDash^I b$.

For any extended arithmetic expression $a \in \mathbf{Aexpv}$, interpretation $I$ and state $\sigma$, it holds that

$$ \mathcal{A}v\llbracket a \rrbracket(I[n/i], \sigma) = \mathcal{A}v\llbracket a[n/i] \rrbracket(I, \sigma) $$

for all integers $n$ and integer variables $i$.

#### Extension

We define the extension of an assertion $A$ w.r.t. an interpretation $I$ to be

$$ A^I \coloneqq \{ \sigma \in \Sigma_\bot \mid \sigma \vDash^I A \}. $$

#### Validity

We say an assertion $A$ is **valid** if for all interpretations $I$ and all states $\sigma$, it holds that

$$ \sigma \vDash^I A. $$

### Partial Correctness Assertions, Revisited

A **partial correctness assertion** is of the form

$$ \{A\}c\{B\}, $$

where $A, B \in \mathbf{Assn}$ and $c \in \mathbf{Com}$.

#### Satisfaction Relation for PCAs

Let $I$ be an interpretation and $\sigma \in \Sigma_\bot$ be a state, we define $\sigma \vDash^I \{A\} c \{ B \}$ iff

$$ \sigma \vDash^I A \Rightarrow \mathcal{C}\llbracket c \rrbracket(\sigma) \vDash^I B. $$

#### Validity of PCAs

- We define $\vDash^I \{ A \} c \{ B \}$ iff $\forall \sigma \in \Sigma_\bot. \sigma \vDash^I \{ A \} c \{ B \}$.
- We define $\vDash\{ A \} c \{ B \}$ iff $\forall I. \vDash^I \{ A \} c \{ B \}$.

A partial correctness assertion is **valid** iff $\vDash\{A\}c\{B\}$.

#### Validity: Assertion vs. PCAs

- $\vDash A \Rightarrow B$ iff $A^I \subseteq B^I$ for all interpretations $I$.
- $\vDash\{A\}c\{B\}$ iff $\mathcal{C}\llbracket c \rrbracket(A^I) \subseteq B^I$ for all interpretations $I$.

## Proof Rules for Partial Correctness Assertions

Manual validation of the validity $\vDash \{A\}c\{B\}$ is tedius. We want to establish some rules to make the proof easier.

### Hoare Rule

#### Skip

$$ \frac{}{\left\{ A \right\} \texttt{skip}\left\{ B \right\}} $$

#### Assignment

$$ \frac{}{\left\{ B[a/X] \right\} X \coloneqq a \left\{ B \right\}} $$

#### Sequential Composition

$$ \frac{\left\{ A \right\} c_0 \left\{ C \right\}, \quad \left\{ C \right\} c_1 \left\{ B \right\}}{\left\{ A \right\} c_0; c_1 \left\{ B \right\}} $$

#### Conditional Branch

$$ \frac{\left\{ A \land b \right\} c_0 \left\{ B \right\}, \quad \left\{ A \land \neg b \right\} c_1 \left\{ B \right\}}{\left\{ A \right\} \texttt{if } b \texttt{ then } c_0 \texttt{ else } c_1 \left\{ B \right\}} $$

#### While Loop

$$ \frac{\left\{ A \land b \right\} c \left\{ A \right\}}{\left\{ A \right\} \texttt{while } a \texttt{ do } c \left\{ A \land \neg b \right\}} $$

- $A$ is called the **loop invariant**.

#### Consequence

$$ \frac{\vDash A \Rightarrow A', \quad \left\{ A' \right\}c\left\{ B' \right\}, \quad \vDash B' \Rightarrow B}{\left\{ A \right\} c \left\{ B \right\}} $$

### Proof System

- Proofs as derivation trees.
- Theorems as conclusion.
- Notion: $\vdash \left\{ A \right\} c \left\{ B \right\}$

## Soundness of Hoare Rules

- **Soundness.** $\vdash \left\{ A \right\} c \left\{ B \right\}$ implies $\vDash \left\{ A \right\} c \left\{ B \right\}$.
  - Every rule should preserve validity. If the assumptions in the rule's premise is valid then so is its conclusion.
- **Completeness.** $\vDash \left\{ A \right\} c \left\{ B \right\}$ implies $\vdash \left\{ A \right\} c \left\{ B \right\}$.
  - We want the proof system to be strong enough so that every valid pca can be obtained as theorems (i.e., provable).

### Proof of Soundness

The proof of soundness depends on some facts about substitution.

**Lemma 1.** Let $I$ be an interpretation, $a, a_0 \in \mathbf{Aexpv}$, $X \in \mathbf{Loc}$. For all interpretations $I$ and states $\sigma$,

$$ Av\llbracket a_0[a/X] \rrbracket(I, \sigma) = Av\llbracket a_0 \rrbracket(I, \sigma[Av\llbracket a \rrbracket(I, \sigma)/X]) $$

*Proof.* By structural induction on $a_0$.

**Lemma 2.** Let $I$ be an interpretation, $B \in \mathbf{Assn}$, $X \in \mathbf{Loc}$, $a \in \mathbf{Aexp}$. For all states $\sigma \in \Sigma$,

$$ \sigma \vDash^I B[a/X] \Longleftrightarrow \sigma[A\llbracket a \rrbracket(\sigma)/X] \vDash^I B.$$

*Proof.* By structural induction on $B$.

#### Ze Proof: By Rule Induction

We show that for every rule instance, if all the extended boolean assertions and pcas in its premises are valid, then so is its conclusion.

> The slide proves via operational semantics, but the textbook mainly uses denotational semantics.

#### Skip

Clearly

$$ \{A\} \texttt{skip} \{A\} $$

so it is sound.

#### Assignment

Assume $c: X \coloneqq a$. By lemma 2 we have

$$\sigma \vDash^I B[a/X] \Longleftrightarrow \sigma[\mathcal{A}\llbracket a \rrbracket(\sigma)/X] \vDash^I B$$

Thus

$$ \sigma \vDash^I B[a/X] \Rightarrow \mathcal{C}\llbracket X \coloneqq a \rrbracket(\sigma) \vDash^I B. $$

by the denotational semantics of $X \coloneqq a$. Hence

$$ \{B[a/X]\} X \coloneqq a \{ B \}. $$

- Recall that
  - $\{A\}c\{B\}$ iff $\sigma \vDash^I A \Rightarrow \mathcal{C}\llbracket c \rrbracket(\sigma) \vDash^I B$.
  - $\mathcal{C}\llbracket X \coloneqq a \rrbracket \coloneqq \{ (\sigma, \sigma[\mathcal{A}\llbracket a \rrbracket(\sigma)/X]) \mid \sigma \in \Sigma \}$.

#### Sequencing

- Assume $\vDash\{A\}c_0\{C\}$ and $\vDash\{C\}c_1\{B\}$.
- Suppose $c \vDash^I A$,
- We have $\mathcal{C}\llbracket c_0 \rrbracket(\sigma) \vDash^I C$ because $\vDash\{A\}c_0\{C\}$.
- Similarly we then have $\mathcal{C}\llbracket c_1 \rrbracket(\mathcal{C}\llbracket c_0 \rrbracket(\sigma)) \vDash^I B$.
- This implies $\vDash \{A\}c_0;c_1\{B\}$.

#### Conditional Branch

- Assume $\vDash \{A \land b\}c_0\{B\}$ and $\vDash \{A \land \neg b\}c_1\{B\}$.
- Suppose $c \vDash^I A$.
- If $\sigma \vDash_I b$, $\sigma \vDash A \land b$ so $\mathcal{C}\llbracket c_0 \rrbracket \vDash^I B$.
- If $\sigma \vDash^I \neg b$, $\sigma \vDash A \land \neg b$ so $\mathcal{C}\llbracket c_1 \rrbracket \vDash^I B$.
- Hence $\sigma \vDash^IA \Rightarrow \mathcal{C}\llbracket \texttt{if } b \texttt{ then } c_0 \texttt{ else } c_1 \rrbracket(\sigma) \vDash^I B$.

#### While Loops

- Assume $\vDash \{A \land b\} c \{A\}$ where $A$ is a loop invariant.
- Denote $w = \texttt{while } b \texttt{ do } c$, $\langle w, \sigma \rangle \to \sigma'$, suppose $\sigma \vDash^I A$.
- If $\langle b, \sigma \rangle \to false$, $\sigma \vDash^I \neg b$ and therefore $\sigma \vDash^I A \land \neg b$.
- If $\langle b, \sigma \rangle \to true$, consider a nested induction on derivation trees,
  $$ \dfrac{\langle b, \sigma \rangle \to true, \quad \langle c, \sigma \rangle \to \sigma'', \quad \langle w, \sigma'' \rangle \to \sigma'}{\langle w, \sigma \rangle \to \sigma'} $$
  - From the main hypothesis, we have $\sigma'' \vDash^I A$ (from $\vDash\{A\land b\}c\{A\}$)
  - From the nested hypothesis, we have $\sigma' \vDash^I A \land \neg b$

This can also be proved with denotational semantics, with the nested induction changed to a mathematical induction on $\theta_n$ (the sequence forming the fixed point of the loop), see textbook.

#### Consequence

- Assume $\vDash A \Rightarrow A'$, $\vDash \{A\}c\{B\}$, $\vDash B' \Rightarrow B$.
- Suppose $\sigma \vDash^I A$, then $\sigma \vDash^I A'$.
- Hence $\mathcal{C}\llbracket c \rrbracket(\sigma) \vDash^I B'$.
- Hence $\mathcal{C}\llbracket c \rrbracket(\sigma) \vDash^I B$.
