# Languages with Higher Types

## A Basic Functional Language

### Syntax

#### Types

The types $\tau$ are generated from the grammar

$$ \tau \coloncolonequals \mathbf{int} \mid \tau_1 * \tau_2 \mid \tau_1 \mapsto \tau_2 $$

- $\mathbf{int}$: the basic type for integers
- $\tau_1 * \tau_2$: product type for ordered pairs
- $\tau_1 \mapsto \tau_2$: function type from $\tau_1$ to $\tau_2$

#### Variables

Let

$$ \mathbf{Var} = \{ x, y, \dots \} $$

denote a st of variables. 


- The function $\mathtt{type}(x)$ returns the uniquely-fixed type for the variable $x$.
- We write $x: \tau$ to stress that $\mathtt{type}(x) = \tau$.

#### Terms

The terms $t$ are generated from the grammar

$$\begin{align*}
    t & \coloncolonequals x &\quad \text{(variable)} \\
    &\mid n \quad &\text{(integer contstants)} \\
    &\mid t_1 \bowtie t_2 \quad (\bowtie \in \{ +, - \times \}) &\quad \text{(arithmetic ops)} \\
    &\mid \texttt{if } t_0 \texttt{ then } t_1 \texttt{ else } t_2  &\\
    &\mid (t_1, t_2) &\quad \text{(ordered pairs)}\\
    &\mid \mathtt{fst}(t) &\quad \text{(first element of ordered pairs)} \\
    &\mid \mathtt{snd}(t) &\quad \text{(second element of ordered pairs)} \\
    &\mid \lambda x.t \\
    &\mid (t_1 \quad t_2) &\quad (\text{function application} t_1(t_2)) \\
    &\mid \texttt{let } x \Leftarrow t_1 \texttt{ in } t_2 &\quad (\text{let notation } t_2[t_1/x])\\
    &\mid \mathtt{rec}y.(\lambda x.t) &\quad (\text{recursion})
\end{align*}$$

### Typing Rules

#### Variables

$$ \dfrac{}{x:\tau} \quad (\mathtt{type}(x) = \tau) $$

#### Arithmetic Ops

$$ \dfrac{}{n : \mathbf{int}} \quad (n \in \mathbb{Z}) $$

$$ \dfrac{t_1: \mathbf{int}, \quad t_2:\mathbf{int}}{t_1 \bowtie t_2: \mathbf{int}} \quad (\bowtie \in \{ +, -, \times \}) $$

The rule requires that arithmetic operations can only be applied to integer types.

#### Conditional Branches

$$ \dfrac{t_0: \mathbf{int}, \quad t_1: \tau, \quad t_2: \tau}{\texttt{if } t_0 \texttt{ then } t_1 \texttt{ else } t_2: \tau} $$

The rule requires that the two branches have the same type $\tau$.

#### Products

$$ \dfrac{t_1: \tau_1, \quad t_2:\tau_2}{(t_1,t_2): \tau_1 * \tau_2} \quad \frac{t: \tau_1 * \tau_2}{\mathtt{fst}(t): \tau_1} \quad \frac{t: \tau_1 * \tau_2}{\mathtt{snd}(t): \tau_2}$$

#### Functions

$$ \dfrac{x: \tau', \quad t: \tau}{\lambda x.t: \tau' \to \tau} \quad \dfrac{t_1: \tau' \to \tau, \quad t_2: \tau'}{(t_1 \quad t_2): \tau} $$

#### Let Notation

$$ \dfrac{x: \tau_1, \quad t_1:\tau_1, \quad t_2:\tau_2}{\texttt{let } x \Leftarrow t_1 \texttt{ in } t_2: \tau_2} $$

#### Recursion

$$ \dfrac{y: \tau, \quad \lambda x.t : \tau}{\mathtt{rec}y.(\lambda x.t): \tau} $$

### Typable Terms

- A term $t$ is **typable** if $t: \tau$ for some type $\tau$.
- A term $t$ is **uniquely typable** if $t: \tau$ for some unique type $\tau$. (i.e., $t: \tau_1$ and $t: \tau_2$ implies $t_1 = t_2$).
- Every typable term is uniquely typable.

### Free Variables

- $FV(n) = \emptyset$
- $FV(x) \coloneqq \{ x \}$
- $FV(t_1 \bowtie t_2) \coloneqq FV(t_1) \cup FV(t_2)$
- $FV(\texttt{if } t_0 \texttt{ then } t_1 \texttt{ else } t_2) \coloneqq FV(t_0) \cup FV(t_1) \cup FV(t_2)$
- $FV((t_1, t_2)) \coloneqq FV((t_1 \quad t_2)) \coloneqq FV(t_1) \cup FV(t_2)$
- $FV(\mathtt{fst}(t)) \coloneqq FV(\mathtt{snd}(t)) \coloneqq FV(t)$
- $FV(\lambda x.t) \coloneqq FV(t) \backslash \{x\}$
- $FV(\texttt{let } x \Leftarrow t_1 \texttt{ in } t_2) \coloneqq FV(t_1) \cup (FV(t_2) \backslash \{x\})$
- $FV(\mathtt{rec}y.(\lambda x.t)) \coloneqq FV(\lambda x.t) \backslash \{y\}$

#### Closed Terms

A term $t$ is closed if $FV(t) = \emptyset$

#### Substitution

Let $t$ be a term, $s$ be a closed term, $x$ be a free variable in $t$. We have

- $t[s/x]$: the term obtained from substituting all free occurrences of $x$ by $s$ in $t$.
- $t[s_1/x_1, \dots, s_k/x_k]$: the term obtained from substituting all free occurrences of $x_i$ by closed terms $s_i$ in $t$.

## Eager Operational Semantics

### Motivating Examples

> To evaluate a function applied to certain arguments we should first evaluate the arguments to obtain values on which the function can then act.

Consider an ordered pair

$$ t = (3+1, (\lambda x.(x+1) \quad 4)) $$

To evaluate $\mathtt{fst}(t)$ eagerly,

1. First we evaluate both $3+1$ and $(\lambda x.(x+1) \quad 4)$
2. Then the final result is the evaluation from $3+1$

Then consider another

$$ t_1 = \lambda x.1, \quad t_2 = (\mathtt{rec}y.(\lambda x.(y \quad x)) \quad 4), \quad t = (t_1 \quad t_2) $$

To evaluate $t$ eagerly, we should evaluate both $t_1$ and $t_2$, and the final result is the function application.

### Canonical Forms (Values)

Let $\tau$ be a type. The set $C_\tau^e$ of **canonical forms** of type $\tau$ is a subset of terms recursively defined as

- $C_{\mathbf{int}}^e \coloneqq \mathbb{Z}$. Numerals are canonical forms.
- $C_{\tau_1 * \tau_2}^{e} \coloneqq C_{\tau_1}^e \times C_{\tau_2}^e$. Pairs of canonical forms are canonical.
- $C_{\tau_1 \to \tau_2}^e \coloneqq \{ \lambda x.t \mid \lambda x.t : \tau_1 \to \tau_2 \text{ is closed (no free variables)} \}$. Closed abstractions are canonical forms.

For any type $\tau$ and term $t \in C_{\tau}^e$, $t$ is closed.

> E.g., $3+5 \notin C_{\mathbf{int}}^e$ but $8 \in C_{\mathbf{int}}^e$.

Intuitively it means we "cannot further simplify the term".

### Evaluation Relation

Let $t$ be a typable closed term with type $\tau$ and $c$ be a canonical term in $C_\tau^e$. Then

$$ t \to^e c $$

denotes $t$ evaluates to $c$ (in eager semantics).

#### Canonical Forms

$$ \dfrac{}{c \to^e c} \quad (c \in C_\tau^e) $$

#### Arithmetic Operations

$$ \dfrac{t_1 \to^e n_1, t_2 \to^e n_2}{(t_1 \bowtie t_2) \to^e n_1 \bowtie n_2} \quad (\bowtie \in\{ +,-,\times\})$$

#### Conditional Branch

$$ \dfrac{t_0 \to^e 0, \quad t_1 \to^e c_1}{\texttt{if } t_0 \texttt{ then } t_1 \texttt{ else } t_2 \to^e c_1} $$

$$ \dfrac{t_0 \to^e n, \quad t_2 \to^e c_2}{\texttt{if } t_0 \texttt{ then } t_1 \texttt{ else } t_2 \to^e c_2} \quad (n\neq 0) $$

where $c_1$ is a canonical form.

Note that some definition for "eager" semantics require that we evaluate all of $t_0,t_1,t_2$.

#### Product

$$ \dfrac{t_1 \to^e c_1, \quad t_2 \to^e c_2}{(t_1,t_2) \to^e (c_1, c_2)} $$

$$ \dfrac{t \to^e (c_1, c_2)}{\mathtt{fst}(t) \to^e c_1} \quad \dfrac{t \to^e (c_1, c_2)}{\mathtt{snd}(t) \to^e c_2} $$

#### Function Application

$$ \dfrac{t_1 \to^e \lambda x.t_1', \quad t_2 \to^e c_2, \quad t_1'[c_2/x] \to^e c}{(t_1 \quad t_2) \to^e c} $$

#### Let Expression

$$ \dfrac{t_1 \to^e c_1, \quad t_2[c_1/x] \to^e c_2}{\texttt{let }x \Leftarrow t_1 \texttt{ in } t_2 \to^e c_2 } $$

#### Recursion

$$ \mathtt{rec}y.(\lambda x.t) \to^e \lambda x.(t[\mathtt{rec}y.(\lambda x.t)/y]) $$

"Replace $y$ with the recursion itself".

### Deterministic Property

- If $t \to^e c$ and $t \to^e c'$ them $c \equiv c'$ (evaluation is deterministic).
- If $t \to^e c$ and $t: \tau$ then $c: \tau$ (evaluation respects types).

## Lazy Operational Semantics

> Only evaluate what is necessary

### A Lazy Language

The syntax of the lazy language is almost the same; the only difference is in the syntax for recursion

$$ \mathtt{rec}x.t $$

where we do not require that $t$ is an abstraction.

#### Typing Rules (Recursion)

$$ \dfrac{y: \tau, \quad t:\tau}{\mathtt{rec}y.t : \tau} $$

### Canonical Forms (Lazy)

Let $\tau$ be a type, the set $C_\tau^l$ is recursively defined as

- $C_\mathbf{int}^l \coloneqq \mathbb{Z}$
- $C_{\tau_1 * \tau_2}^l \coloneqq \{ (t_1, t_2) \mid t_1 : \tau_1, t_2 : \tau_2, \quad t_1, t_2\text{ are closed} \}$
- $C_{\tau_1 \to \tau_2}^l \coloneqq \{ \lambda x.t \mid \lambda x.t : \tau_1 \to \tau_2 \text{ is closed} \}$

### The Evaluation Relation (Lazy)

$$ t \to^l c $$

denotes $t$ evaluates to $c$ in lazy operational semantics

#### Canonical Terms

$$ \dfrac{}{c \to^l c} \quad (c \in C_\tau^l) $$

#### Arithmetic Operations

$$ \dfrac{t_1 \to^l n_1, t_2 \to^l n_2}{(t_1 \bowtie t_2) \to^l n_1 \bowtie n_2} \quad (\bowtie \in\{ +,-,\times\})$$

#### Conditional Branch

$$ \dfrac{t_0 \to^l 0, \quad t_1 \to^l c_1}{\texttt{if } t_0 \texttt{ then } t_1 \texttt{ else } t_2 \to^l c_1} $$

$$ \dfrac{t_0 \to^l n, \quad t_2 \to^l c_2}{\texttt{if } t_0 \texttt{ then } t_1 \texttt{ else } t_2 \to^l c_2} \quad (n\neq 0) $$

#### Product

$$ \dfrac{t_1 \to^l c_1, \quad t_2 \to^l c_2}{(t_1,t_2) \to^l (c_1, c_2)} $$

$$ \dfrac{t \to^l (t_1, t_2), \quad t_1 \to^l c_1}{\mathtt{fst}(t) \to^l c_1} \quad \dfrac{t \to^l (t_1, t_2), \quad t_2 \to^l c_2}{\mathtt{snd}(t) \to^l c_2} $$

#### Function Application

$$ \dfrac{t_1 \to^l \lambda x.t_1', \quad t_1'[t_2/x] \to^l c}{(t_1 \quad t_2) \to^l c} $$

#### Let Expression

$$ \dfrac{t_2[t_1/x] \to^l c}{\texttt{let }x \Leftarrow t_1 \texttt{ in } t_2 \to^l c } $$

#### Recursion

$$ \dfrac{t[\mathtt{rec}y.t/y] \to^l c}{\mathtt{rec}y.t \to^l c} $$

### Deterministic and Respect Type (Lazy)

Lazy semantics is also deterministic and respects types

- If $t \to^l c$ and $t \to^l c'$ then $c \equiv c'$
- If $t \to^l c$ and $t: \tau$ then $c: \tau$.

## Eager Denotational Semantics

### Values

Let $\tau$ be a type, the cpo $V_\tau^e$ of **values** associated with the type $\tau$ is recursively defined as

- $V_\mathbf{int}^e \coloneqq \mathbb{Z}$ (discrete cpos)
- $V_{\tau_1 * \tau_2}^e \coloneqq V_{\tau_1}^e \times V_{\tau_2}^e$ (product cpo)
- $V_{\tau_1 \to \tau_2}^e \coloneqq [V_{\tau_1}^e \to (V_{\tau_2}^e)_\bot]$ (function space)

The $\bot$ in the final clause captures the idea that a function value takes a value as input and delivers a value as output or diverges.

### Environment

Terms typically contain free variables, and we use the notion of environment to supply values to free variables. An **environment** is typically a function

$$ \rho: \mathbf{Var} \to \bigcup\left\{ V_\tau^e \mid \tau \text{ is a type} \right\} $$

such that

$$ \forall x \in \mathbf{Var}.(x: \tau \Rightarrow \rho(x) \in V_{\tau}^e) $$

### Denotational Semantics

#### Intuition

Let $t$ be a typable term with type $\tau$, $\llbracket t \rrbracket^e: \mathbf{Env} \to (V_\tau^e)_\bot$ be the denotational semantics of $t$

#### Denotational Semantics by Structural Induction

- $\llbracket x \rrbracket^e \coloneqq \lambda \rho.\lfloor \rho(x) \rfloor$
- $\llbracket n \rrbracket^e \coloneqq \lambda \rho.\lfloor n \rfloor$
- $\llbracket t_1 \bowtie t_2 \rrbracket^e \coloneqq \lambda\rho.(\llbracket t_1 \rrbracket^e(\rho) \bowtie_\bot \llbracket t_2 \rrbracket^e(\rho))$
- $\llbracket \texttt{if } t_0 \texttt{ then } t_1 \texttt{ else } t_2 \rrbracket^e \coloneqq \lambda\rho.\mathtt{cond}(\llbracket t_0 \rrbracket^2(\rho), \llbracket t_1 \rrbracket^e(\rho), \llbracket t_2 \rrbracket^e(\rho))$
- $\llbracket \mathtt{fst}(t) \rrbracket^e \coloneqq \lambda\rho.\texttt{let }v \Leftarrow \llbracket t \rrbracket^e(\rho).\lfloor \pi_1(v) \rfloor$
- $\llbracket \mathtt{snd}(t) \rrbracket^e \coloneqq \lambda\rho.\texttt{let }v \Leftarrow \llbracket t \rrbracket^e(\rho).\lfloor \pi_2(v) \rfloor$
- $\llbracket (t_1, t_2) \rrbracket^e \coloneqq \lambda\rho.\texttt{let }v_1\Leftarrow \llbracket t_1 \rrbracket^e(\rho), v_2\Leftarrow \llbracket t_2 \rrbracket^e(\rho).\lfloor (v_1, v_2) \rfloor$
- $\llbracket \lambda x.t \rrbracket^e \coloneqq \lambda\rho.\lfloor \lambda v\in V_{\tau_1}^e.\llbracket t \rrbracket^e\rho\llbracket v/x \rrbracket \rfloor$ where $\lambda x.t : \tau_1 \to \tau_2$
- $\llbracket (t_1 \quad t_2) \rrbracket^e \coloneqq \texttt{let }F \Leftarrow \llbracket t_1 \rrbracket^e(\rho), v\Leftarrow \llbracket t_2 \rrbracket^e(\rho).F(v)$
- $\llbracket \texttt{let }x \Leftarrow t_1 \texttt{ in } t_2  \rrbracket^e \coloneqq \lambda \texttt{let }v \Leftarrow \llbracket t_1 \rrbracket^e(\rho).\llbracket t_2 \rrbracket^e(\rho[v/x])$
- $\llbracket \mathtt{rec}y.(\lambda x.t) \rrbracket^e \coloneqq \lambda\rho.\lfloor \mu F.(\lambda v.\llbracket t \rrbracket^e(\rho[v/x, F/y])) \rfloor$

#### Function Update

- $in_1: \{x\} \to \mathbf{Var}: x \mapsto x$
- $in_2: \mathbf{Var} \backslash \{x\} \to \mathbf{Var}: y \mapsto y, y \neq x$

$$ \rho[v/x](y) = \begin{cases}
    v &\quad y = x\\
    \rho(y) &\quad y \neq x
\end{cases} $$

$$ \rho[v/x] = \lambda y.\texttt{case } y \texttt{ of } in_1(y_1).v \mid in_2(y_2).\rho(y_2) $$

### Substitution Lemma

**Lemma.** Let $t$ be a typable term, $\rho, \rho'$ be environments which agree on the free variables of $t$. Then

$$ \llbracket t \rrbracket^e(\rho) = \llbracket t \rrbracket^e (\rho') $$

The value assignment of non-free variable will not affect the final result.

**Lemma (Substitution Lemma).** Let $s$ be a closed term with $s: \tau$ such that $\llbracket s \rrbracket^e(\rho) = \lfloor v \rfloor$. Let $x$ be a variable with $x : \tau$ and $t$ be a term with $t: \tau'$, then

- $t[s/x] : \tau'$
- $\llbracket t[s/x] \rrbracket^e(\rho) = \llbracket t \rrbracket^e(\rho[v/x])$

**Another Lemma.** If $t: \tau$ then for all $\rho$ we have $\llbracket t \rrbracket^e(\rho)\in(V_\tau^e)_\bot$.

**Yet Another Lemma.** If $c \in C_\tau^e$ then for all $\rho$ we have $\llbracket c \rrbracket^e(\rho) \neq \bot$ (the bottom element for $(V_\tau^e)_\bot$)

- A canonical form will not diverge under denotational semantics.

## Agreement of Eager Semantics

Ideally we would expect

$$ t \to^e c \Longleftrightarrow \llbracket t \rrbracket^e(\rho) = \llbracket c \rrbracket^e(\rho). $$

It can be shown that LHS to RHS holds, but RHS to LHS might not hold.

The correct statement should be:

Let $t$ be a closed typable term and $c$ be a canonical form. We have

- $t \to^e c$ implies $\llbracket t \rrbracket^e(\rho) = \llbracket c \rrbracket^e(\rho)$
- The two eager semantics agree on the *convergence* of $t$.

### Convergence

#### Operational Convergence

Let $t$ be a typable closed term. We say that $t$ is **operationally convergent**, denoted by $t \downarrow^e$ if it holds that $\exists c.t \to^e c$.

#### Denotational Convergence

Let $t$ be a typable closed term with type $\tau$. We say that $tg$ is **denotationally convergent**, denoted by $t \Downarrow^e$ if it holds that $\exists v \in V_\tau^e.\llbracket t \rrbracket^e(\rho) = \lfloor v \rfloor$.

Intuitively it means we can find such a value $v$ s.t. $t$ is evaluated to the lifting of $v$.

### Agreement of Eager Semantics

Let $t$ be a closed typable term and $c$ be a canonical form. We have

- $t \to^e c$ implies $\llbracket t \rrbracket^e(\rho) = \llbracket c \rrbracket^e(\rho)$
- $t \downarrow^e$ iff $t \Downarrow^e$

### Corollary

Let $t$ be a closed typable term with type $\mathbf{int}$. We have

$$ t \to^e c \Longleftrightarrow \llbracket t \rrbracket^e(\rho) = \llbracket c \rrbracket^e(\rho). $$

Basically it states that if the type is int, we can have the equivalence between operational and denotational semantics. However, in general, this does not hold.

### Final Notes

- The Lazy Denotational Semantics and the agreement of lazy semantics are defined similarly.
